Add support for PUSHXX bytecodes #117 #21
This adds support for (in principle) the full variety of PUSH bytecodes.
However, there are some dragons.  In particular, the map used within
EvmBerlin does not verify with the full set of bytecodes.  I think we
are hitting some kind of EVM limit here, though it is hard to say.

src/dafny/util/int.dfy
@@ -17,8 +17,12 @@ module Int {
   const TWO_8   : int := 0x1_00;
   const TWO_15  : int := 0x0_8000;
   const TWO_16  : int := 0x1_0000;
+  const TWO_24  : int := 0x1_0000_00;
   const TWO_31  : int := 0x0_8000_0000;
   const TWO_32  : int := 0x1_0000_0000;
+  const TWO_40  : int := 0x1_0000_0000_00;
+  const TWO_48  : int := 0x1_0000_0000_0000;
+  const TWO_56  : int := 0x1_0000_0000_0000_00;
   const TWO_63  : int := 0x0_8000_0000_0000_0000;
   const TWO_64  : int := 0x1_0000_0000_0000_0000;
   const TWO_127 : int := 0x0_8000_0000_0000_0000_0000_0000_0000_0000;
@@ -51,7 +55,11 @@ module Int {
   // Unsigned Integers
   const MAX_U8 : int :=  TWO_8 - 1;
   const MAX_U16 : int := TWO_16 - 1;
+  const MAX_U24 : int := TWO_24 - 1;
   const MAX_U32 : int := TWO_32 - 1;
+  const MAX_U40 : int := TWO_40 - 1;
+  const MAX_U48 : int := TWO_48 - 1;
+  const MAX_U56 : int := TWO_56 - 1;
   const MAX_U64 : int := TWO_64 - 1;
   const MAX_U128 : int := TWO_128 - 1;
   const MAX_U160: int := TWO_160 - 1;
@@ -59,7 +67,11 @@ module Int {
 
   newtype{:nativeType "byte"} u8 = i:int    | 0 <= i <= MAX_U8
   newtype{:nativeType "ushort"} u16 = i:int | 0 <= i <= MAX_U16
+  newtype{:nativeType "uint"} u24 = i:int | 0 <= i <= MAX_U24
   newtype{:nativeType "uint"} u32 = i:int   | 0 <= i <= MAX_U32
+  newtype{:nativeType "ulong"} u40 = i:int   | 0 <= i <= MAX_U40
+  newtype{:nativeType "ulong"} u48 = i:int   | 0 <= i <= MAX_U48
+  newtype{:nativeType "ulong"} u56 = i:int   | 0 <= i <= MAX_U56
   newtype{:nativeType "ulong"} u64 = i:int  | 0 <= i <= MAX_U64
   newtype u128 = i:int | 0 <= i <= MAX_U128
   newtype u160 = i:int | 0 <= i <= MAX_U160
@@ -95,6 +107,41 @@ module Int {
     (b1 * (TWO_32 as u64)) + b2
   }
 
+  // =========================================================
+  // Exponent
+  // =========================================================
+
+  /**
+   * Compute n^k.
+   */
+  function method Pow(n:int, k:nat) : int
+  requires k > 0 {
+    if k == 1 then n
+    else
+      n * Pow(n,k-1)
+  }
+
+  // Various sanity tests for exponentiation.
+  method PowTests() {
+    assert Pow(2,8) == TWO_8;
+    assert Pow(2,15) == TWO_15;
+    assert Pow(2,16) == TWO_16;
+    assert Pow(2,24) == TWO_24;
+    assert Pow(2,31) == TWO_31;
+    assert Pow(2,32) == TWO_32;
+    assert Pow(2,40) == TWO_40;
+    assert Pow(2,48) == TWO_48;
+    assert Pow(2,56) == TWO_56;
+    assert Pow(2,63) == TWO_63;
+    assert Pow(2,64) == TWO_64;
+    // NOTE:  I have to break the following ones up because Z3
+    // cannot handle it.
+    assert Pow(2,63) * Pow(2,64) == TWO_127;
+    assert Pow(2,64) * Pow(2,64) == TWO_128;
+    assert Pow(2,64) * Pow(2,64) * Pow(2,64) * Pow(2,64) == TWO_256;
+    assert (TWO_128 / TWO_64) == TWO_64;
+    assert (TWO_256 / TWO_128) == TWO_128;
+  }
 
   // =========================================================
   // Non-Euclidean Division / Remainder
